Liveness: refactored start of the proof and modified form of the states in proof

Graphiti/Projects/Liveness/ComposedLiveness.lean
@@ -20,166 +20,6 @@ import Graphiti.Core.Trace
 open Graphiti
 open Graphiti.Module
 open List
--- namespace Module
--- namespace NatModule
-
--- #check NatModule.gfmodule
-
--- if `f(x)` is in the module, then it can be output (through steps `t'`, leading to new state `s'` which is empty)
-/-
-lemma gcompf_flushability {T} (f g: T → T):
-  ∀ (x: T) (s: State _ _), s.module = (NatModule.gcompf T f g) ∧ (f x) ∈ s.state.fst
-  → ∃ t' s', (@star _ _ (state_transition s.module) ⟨s.state,  s.module⟩ t' ⟨s', s.module⟩)
-  ∧ .output 0 ⟨ T, g (f x) ⟩ ∈ t'
-  ∧ s' = (∅, ∅) := by
-    intros x s h
-    have ⟨ h1, h2 ⟩ := h
-    -- step internal, get s2 with internal state (∅, ∀x∈s -> g(f(x)))
-    have h_int: ∃ s2, step s [] ⟨s2, s.module⟩ := by rw [h1]; sorry -- use h2
-    -- step output
-    have h_out: ∃ s3 v', step s [.output 0 v'] ⟨s3, s.module⟩ := by sorry
-    -- gotta prove that v' = g(f(x)) and that s3 = s'
-    sorry
-
-
-lemma gcompfp_lemma2 {t t': Trace Nat} {T f g} : -- rename it to `gcompf_stuck_input` ?
-  ∀ x (s: State _ _) s', s.module = (NatModule.gcompf T f g)
-  -- ∧ @reachable _ _ (state_transition s.module) t' s
-  ∧ @star _ _ (state_transition s.module) s t s'
-  ∧ .input 0 ⟨ T, x ⟩ ∈ t ∧ .output 0 ⟨ T, g (f x) ⟩ ∉ t
-  → (f x) ∈ s.state.fst ∨ g (f x) ∈ s.state.snd := by
-    sorry
-
--- if some input `x` was fed to g∘f module, but output `g(f(x))` is not out, then `x` is currently *in* the module, either in the first list (as `f(x)`) or in the second list (as `g(f(x))`)
-lemma gcompfp_lemma {t t0: Trace Nat} {T f g} : -- rename it to `gcompf_stuck_input` ?
-  ∀ x (s: State _ _) s', @star _ _ (state_transition s.module) s t s'
-  → s.module = (NatModule.gcompf T f g)
-  → @reachable _ _ (state_transition s.module) t0 s
-  → .input 0 ⟨ T, x ⟩ ∈ (t0 ++ t) → .output 0 ⟨ T, g (f x) ⟩ ∉ (t0 ++ t)
-  → (f x) ∈ s.state.fst ∨ g (f x) ∈ s.state.snd := by
-    -- try to get away from beh asap, so you don't have to start at init state which is empty since we can't induct over that
-    intros x s s' h
-    revert x t0
-    generalize heq: state_transition s.module = n at * -- will need to prove that module stays constant (exist lemma)
-    induction h
-    case refl => sorry
-    case step => sorry
-
-
-
-
-
-def gcompf_P {T} (t: Trace Nat)(f g: T → T) : Prop :=
-  ∀ in1, .input 0 ⟨ T, in1 ⟩ ∈ t → .output 0 ⟨ T, g (f (in1)) ⟩ ∈ t
-
---theorem gcompf_inp {T f g} : ∀ t t0 x, .input 0 ⟨T, x ⟩ ∉ t0 ∧ gcompf_P (t ++ t0) f g ∧ ∃ s s0, @star _ _ (state_transition s.module) s t0 s0
---:= by sorry
-
-theorem gcompf_reachness {T f g} : ∀ t s s', @star _ _ (state_transition (NatModule.gcompf T f g)) s t s'
-  → ∀ t0, (∀ x, .input 0 ⟨ T, x ⟩ ∉ t0)
-  → gcompf_P (t ++ t0) f g
-  → ∀ e s'', @star _ _ (state_transition (NatModule.gcompf T f g)) s' [e] s''
-  → ∃ sn tn,gcompf_P (t ++ [e] ++ tn) f g ∧ @star _ _ (state_transition (NatModule.gcompf T f g)) s'' tn sn ∧ ∀ x, .input 0 ⟨T, x ⟩ ∉ tn:= by sorry
-
-
--- if 0 steps holds, if n steps have to check the reachabilty + */// lemmas: is input included, is output included
--- with module gcompf, if "in1" in trace α, then there exist a β where eventually "out1 = g∘f(in1)" in trace αβ
-theorem gcompf_liveness {t : Trace Nat} {T f g} (h_steps: @behaviour _ _ (state_transition (NatModule.gcompf T f g)) t)  :
-  ∃ t', gcompf_P (t ++ t') (f) (g) ∧ @behaviour _ _ (state_transition (NatModule.gcompf T f g)) (t ++ t') ∧ ∀ x, .input 0 ⟨T, x⟩ ∉ t' := by
-    cases h_steps
-    rename_i s1 behUnfolded
-    have helpNext := (s1.module.state_transition = (state_transition (NatModule.gcompf T f g)))
-    cases behUnfolded
-    rename_i s2 behUnfolded
-    have starRevConv := (@star_eq_star_rev _ _ (state_transition (NatModule.gcompf T f g)) s1 s2 t).mp behUnfolded.right
-    induction starRevConv
-    . exists []
-      simp [gcompf_P]
-      exists s1
-      exists s1
-    . rename_i s3 s4 l1 l2 stepP starP iH
-      have starConv := (@star_eq_star_rev _ _ (state_transition (NatModule.gcompf T f g)) s1 s3 l1).mpr starP
-      have iHEval := iH (And.intro behUnfolded.left starConv)
-      cases iHEval
-      clear iH
-      rename_i l2 iH
-      have stepPP := stepP
-      cases stepP
-      . rename_i ip LxL firstInputV firstInputTpe secondInputV firstInputEq
-        have behConv := iH.right.left
-        simp [behaviour_tight] at behConv
-        cases behConv
-        rename_i s4 behConv
-        cases behConv
-        rename_i s5 behConv
-        cases behConv
-        rename_i stateInits5 cc
-        have lemmaUse :=  @gcompf_reachness T f g
-        simp [reachable] at lemmaUse
-        have stepToStar := @star.plus_one _ _ (state_transition (NatModule.gcompf T f g)) s3 ({ state := LxL, module := s3.module }) ([IOEvent.input ip firstInputTpe]) stepPP
-        have lemmaUse1 := lemmaUse l1 s1 s3 starConv l2 iH.right.right iH.left (IOEvent.input ip firstInputTpe) ({ state := LxL, module := s3.module }) stepToStar
-        cases lemmaUse1
-        rename_i s6 lemma1
-        cases lemma1
-        rename_i l3 indLemma
-        exists l3
-        constructor
-        . simp at *
-          exact indLemma.left
-        . constructor
-          . simp [behaviour]
-            exists s1
-            constructor
-            . exact behUnfolded.left
-            . clear lemmaUse
-              exists s6
-              have firstSteps := @star.trans_star _ _ (state_transition (NatModule.gcompf T f g)) s1 s3 ({ state := LxL, module := s3.module }) l1 [IOEvent.input ip firstInputTpe] starConv
-              have firstSteps1 := firstSteps stepToStar
-              have secondSteps := @star.trans_star _ _ (state_transition (NatModule.gcompf T f g)) s1 { state := LxL, module := s3.module } s6 (l1 ++ [IOEvent.input ip firstInputTpe]) l3 firstSteps1 indLemma.right.left
-              simp at *
-              assumption
-          . exact indLemma.right.right
-      . rename_i ip LxL firstInputV firstInputTpe secondInputV firstInputEq
-        have behConv := iH.right.left
-        simp [behaviour_tight] at behConv
-        cases behConv
-        rename_i s4 behConv
-        cases behConv
-        rename_i s5 behConv
-        cases behConv
-        rename_i stateInits5 cc
-        have lemmaUse :=  @gcompf_reachness T f g
-        simp [reachable] at lemmaUse
-        have stepToStar := @star.plus_one _ _ (state_transition (NatModule.gcompf T f g)) s3 ({ state := LxL, module := s3.module }) ([IOEvent.output ip firstInputTpe]) stepPP
-        have lemmaUse1 := lemmaUse l1 s1 s3 starConv l2 iH.right.right iH.left (IOEvent.output ip firstInputTpe) ({ state := LxL, module := s3.module }) stepToStar
-        cases lemmaUse1
-        rename_i s6 lemma1
-        cases lemma1
-        rename_i l3 indLemma
-        exists l3
-        constructor
-        . simp at *
-          exact indLemma.left
-        . constructor
-          . simp [behaviour]
-            exists s1
-            constructor
-            . exact behUnfolded.left
-            . clear lemmaUse
-              exists s6
-              have firstSteps := @star.trans_star _ _ (state_transition (NatModule.gcompf T f g)) s1 s3 ({ state := LxL, module := s3.module }) l1 [IOEvent.output ip firstInputTpe] starConv
-              have firstSteps1 := firstSteps stepToStar
-              have secondSteps := @star.trans_star _ _ (state_transition (NatModule.gcompf T f g)) s1 { state := LxL, module := s3.module } s6 (l1 ++ [IOEvent.output ip firstInputTpe]) l3 firstSteps1 indLemma.right.left
-              simp at *
-              assumption
-          . exact indLemma.right.right
-      . rename_i RLL LL RLLInS3 RLLS
-        exists l2
-        simp at *
-        assumption
--/
-
-
 
 /-
 New approach: using behaviours is too limiting, I decided to do a secondary proof exclusively on star and prove behaviour
@@ -284,45 +124,32 @@ theorem gcompf_reachness_empty {T f g} : ∀ t s', @reachable _ _ (state_transit
     exists l5
 
 
-
-theorem gcompf_reachness_input {T f g} : ∀ t s', @reachable _ _ (state_transition (NatModule.gcompf T f g)) t s'
-→ ∀ s'' t0, ( ∀ x, .input 0 ⟨ T, x ⟩ ∉ t0) ∧ @star _ _ (state_transition (NatModule.gcompf T f g)) s' t0 s''
+theorem gcompf_reachness_input { T f g} (s1 s2 s3 : List T × List T) (t t0: List (IOEvent ℕ)) (io: T): @reachable _ _ (state_transition (NatModule.gcompf T f g)) t  ⟨ s1, (NatModule.gcompf T f g)⟩
+→ ( ∀ x, .input 0 ⟨T, x⟩ ∉ t0) ∧ @star _ _ (state_transition (NatModule.gcompf T f g)) ⟨ s1, (NatModule.gcompf T f g)⟩ t0 ⟨s2, (NatModule.gcompf T f g )⟩
 → gcompf_P (t ++ t0) f g
-→ ∀ x s''', @step _ _ _ s' [IOEvent.input 0 ⟨T, x⟩] s'''
-→ ∃ sn tn, gcompf_P (t ++ [IOEvent.input 0 ⟨T, x⟩] ++ tn) f g ∧ @star _ _ (state_transition (NatModule.gcompf T f g)) s''' tn sn ∧ ∀ x, .input 0 ⟨T, x ⟩ ∉ tn:= by
-  intro l1 s1 reachP s2 l2  noInpiInL2 gcomfProp io s3 step
+→ @step _ _ _ ⟨ s1, (NatModule.gcompf T f g)⟩ [IOEvent.input 0 ⟨ T, io⟩]  ⟨s3, (NatModule.gcompf T f g) ⟩
+→ ∃ sn tn, gcompf_P (t ++ [IOEvent.input 0 ⟨T, io ⟩] ++ tn) f g ∧ @star _ _ (state_transition (NatModule.gcompf T f g)) ⟨ s3, (NatModule.gcompf T f g) ⟩  tn sn ∧ ∀ x, .input 0 ⟨T, x ⟩ ∉ tn:= by
   sorry
 
-/--
-theorem gcompf_reachness_output { T f g} : ∀ t s', @reachable _ _ (state_transition (NatModule.gcompf T f g)) t  ⟨ s', (NatModule.gcompf T f g)⟩
-→ ∀ s'' t0 ,( ∀ x, .input 0 ⟨T, x ⟩ ∉ t0) ∧ @star _ _ (state_transition (NatModule.gcompf T f g)) ⟨ s', (NatModule.gcompf T f g)⟩ t0 s''
+
+
+
+theorem gcompf_reachness_output { T f g} (s1 s2 s3 : List T × List T) (t t0: List (IOEvent ℕ)) (io: T): @reachable _ _ (state_transition (NatModule.gcompf T f g)) t  ⟨ s1, (NatModule.gcompf T f g)⟩
+→ ( ∀ x, .input 0 ⟨T, x⟩ ∉ t0) ∧ @star _ _ (state_transition (NatModule.gcompf T f g)) ⟨ s1, (NatModule.gcompf T f g)⟩ t0 ⟨s2, (NatModule.gcompf T f g )⟩
 → gcompf_P (t ++ t0) f g
-→ ∀ io s''', @step _ _ _ ⟨ s', (NatModule.gcompf T f g)⟩ [IOEvent.output 0 ⟨ T, io⟩]  s'''
-→ ∃ sn tn, gcompf_P (t ++ [IOEvent.output 0 ⟨T, io ⟩] ++ tn) f g ∧ @star _ _ (state_transition (NatModule.gcompf T f g)) s''' tn sn ∧ ∀ x, .input 0 ⟨T, x ⟩ ∉ tn:= by
-  intro l1 s1 reachP s2 l2 noInpiInL2 gcomfProp io s3 step
-  cases step
-  rename_i s' v a a'
-  simp at *
-  rw [PortMap.rw_rule_execution (by simp [drunfold]; rfl)] at *
+→ @step _ _ _ ⟨ s1, (NatModule.gcompf T f g)⟩ [IOEvent.output 0 ⟨ T, io⟩]  ⟨s3, (NatModule.gcompf T f g) ⟩
+→ ∃ sn tn, gcompf_P (t ++ [IOEvent.output 0 ⟨T, io ⟩] ++ tn) f g ∧ @star _ _ (state_transition (NatModule.gcompf T f g)) ⟨ s3, (NatModule.gcompf T f g) ⟩  tn sn ∧ ∀ x, .input 0 ⟨T, x ⟩ ∉ tn:= by
   sorry
--/
-theorem gcompf_reachness_output { T f g} : ∀ t s', @reachable _ _ (state_transition (NatModule.gcompf T f g)) t  s'
-→ ∀ s'' t0 ,( ∀ x, .input 0 ⟨T, x ⟩ ∉ t0) ∧ @star _ _ (state_transition (NatModule.gcompf T f g)) s' t0 s''
-→ gcompf_P (t ++ t0) f g
-→ ∀ io s''', @step _ _ _ s' [IOEvent.output 0 ⟨ T, io⟩]  s'''
-→ ∃ sn tn, gcompf_P (t ++ [IOEvent.output 0 ⟨T, io ⟩] ++ tn) f g ∧ @star _ _ (state_transition (NatModule.gcompf T f g)) s''' tn sn ∧ ∀ x, .input 0 ⟨T, x ⟩ ∉ tn:= by
-  intro l1 s1 reachP s2 l2 noInpiInL2 gcomfProp io s3 step
-  cases step
-  rename_i s' v a a'
-  simp at *
-  rw [PortMap.rw_rule_execution (by simp [drunfold]; rfl)] at *
-  sorry
+
+
 
 
 theorem gcompf_liveness_simp {t : Trace Nat} {T f g}
 (h_in: (∀ G x n, IOEvent.input n ⟨G, x⟩  ∈ t → (n = 0) ∧ G = T))
 (h_out: (∀ G x n, IOEvent.output n ⟨G, x⟩  ∈ t → (n = 0) ∧ G = T))
 (s1 s2: State _ _)
+(h_s1: s1.module = (NatModule.gcompf T f g))
+(h_s2: s2.module = (NatModule.gcompf T f g))
 (h: @StateTransition.init _ _ (state_transition (NatModule.gcompf T f g)) s1 ∧ @star _ _ (state_transition (NatModule.gcompf T f g)) s1 t s2):
   ∃ t' s3, gcompf_P (t ++ t') f g ∧ @star _ _ (state_transition (NatModule.gcompf T f g)) s2 t' s3 ∧ (∀ x, .input 0 ⟨T, x⟩ ∉ t'):= by
     have starConv := (@star_eq_star_rev _ _ (state_transition (NatModule.gcompf T f g)) s1 s2 t).mp h.right
@@ -349,7 +176,9 @@ theorem gcompf_liveness_simp {t : Trace Nat} {T f g}
         constructor
         assumption
       }
-      have iHRes := iH h_in_new h_out_new (And.intro h.left starConv)
+      have keep := steps_preserve_mod (NatModule.gcompf T f g) starConv
+      rw [h_s1] at keep
+      have iHRes := iH h_in_new h_out_new keep (And.intro h.left starConv)
       clear iH
       cases iHRes
       rename_i tr iH
@@ -357,19 +186,24 @@ theorem gcompf_liveness_simp {t : Trace Nat} {T f g}
       rename_i s5 iH
       have keepStep := step
       cases step
-      . rename_i IntN LTPair s3Fst TT s3Snd TTEq
-        have finalRes := @gcompf_reachness_input T f g l1 s3
-        simp [reachable] at finalRes
-        have finalResT := finalRes s1 h.left starConv s5 tr iH.right.right iH.right.left iH.left
+      . rename_i IntN s4 s3Fst TT s3Snd TTEq
+        cases s3
+        rename_i s3 mod3
+        subst keep
+        have finalResT := @gcompf_reachness_input T f g
+        simp [reachable] at finalResT
+        cases s5
+        rename_i s5 mod5
         cases TT
         rename_i TT inp
         have h_in_assum := h_in TT inp IntN
         simp at h_in_assum
-        clear finalRes
         rcases h_in_assum with ⟨ nEq, TypeEq ⟩
         subst nEq
         subst TypeEq
-        have finalRes := finalResT inp { state := LTPair, module := s3.module } keepStep
+        have s5_mod_eq := steps_preserve_mod (NatModule.gcompf TT f g) iH.right.left
+        subst s5_mod_eq
+        have finalRes := finalResT s3.1 s3.2 s5.1 s5.2 s4.1 s4.2 l1 tr inp s1 h.left starConv iH.right.right iH.right.left iH.left keepStep
         cases finalRes
         rename_i s4 finalRes
         cases finalRes
@@ -378,19 +212,24 @@ theorem gcompf_liveness_simp {t : Trace Nat} {T f g}
         exists s4
         simp at *
         exact final
-      . rename_i IntN LTPair s3Fst TT s3Snd TTEq
-        have finalRes :=@ gcompf_reachness_output T f g l1 s3
-        simp [reachable] at finalRes
-        have finalResT := finalRes s1 h.left starConv s5 tr iH.right.right iH.right.left iH.left
+      . rename_i IntN s4 s3Fst TT s3Snd TTEq
+        cases s3
+        rename_i s3 mod3
+        subst keep
+        have finalResT := @gcompf_reachness_output T f g
+        simp [reachable] at finalResT
+        cases s5
+        rename_i s5 mod5
         cases TT
         rename_i TT inp
         have h_out_assum := h_out TT inp IntN
         simp at h_out_assum
-        clear finalRes
         rcases h_out_assum with ⟨ nEq, TypeEq ⟩
         subst nEq
         subst TypeEq
-        have finalRes := finalResT inp { state := LTPair, module := s3.module } keepStep
+        have s5_mod_eq := steps_preserve_mod (NatModule.gcompf TT f g) iH.right.left
+        subst s5_mod_eq
+        have finalRes := finalResT s3.1 s3.2 s5.1 s5.2 s4.1 s4.2 l1 tr inp s1 h.left starConv iH.right.right iH.right.left iH.left keepStep
         cases finalRes
         rename_i s4 finalRes
         cases finalRes
@@ -418,29 +257,27 @@ theorem gcompf_liveness_simp {t : Trace Nat} {T f g}
 
 
 theorem gcompf_liveness2 {t : Trace Nat} {T f g}(h_steps: @behaviour _ _ (state_transition (NatModule.gcompf T f g)) t)
-(h_in: (∀ G x n, IOEvent.input n ⟨G, x⟩  ∈ t → (n = 0) ∧ G = T))
-(h_out: (∀ G x n, IOEvent.output n ⟨G, x⟩  ∈ t → (n = 0) ∧ G = T)):
+(h_input: (∀ G x n, IOEvent.input n ⟨G, x⟩  ∈ t → (n = 0) ∧ G = T))
+(h_output: (∀ G x n, IOEvent.output n ⟨G, x⟩  ∈ t → (n = 0) ∧ G = T))
+(h_init_imp_mod: ∀s, @StateTransition.init _ _ (state_transition (NatModule.gcompf T f g)) s  → s.module = (NatModule.gcompf T f g)):
   ∃ t', gcompf_P (t ++ t') (f) (g) ∧ @behaviour _ _ (state_transition (NatModule.gcompf T f g)) (t ++ t') ∧ ∀ x, .input 0 ⟨T, x⟩ ∉ t' := by
     simp [behaviour] at h_steps
-    cases h_steps
-    rename_i s1 beh
-    cases beh
-    rename_i p1 beh
-    cases beh
-    rename_i s2 star
-    have mainProof := gcompf_liveness_simp h_in h_out s1 s2 (And.intro p1 star)
-    cases mainProof
-    rename_i t' mainProof
-    cases mainProof
-    rename_i s3 mainProof
-    exists t'
-    constructor
-    . exact mainProof.left
-    . constructor
-      . simp [behaviour]
-        have starComb := @star.trans_star _ _ (state_transition (NatModule.gcompf T f g)) s1 s2 s3 t t' mainProof.right.left
-        exists s1
+    match h_steps with
+    | ⟨ s1, s1_init_step, s2, s1_star_s2_t ⟩  =>
+      have s1_mod_eq := h_init_imp_mod s1 s1_init_step
+      have s2_mod_eq := steps_preserve_mod (NatModule.gcompf T f g) s1_star_s2_t
+      rw [s1_mod_eq] at s2_mod_eq
+      have induct_star_res := gcompf_liveness_simp h_input h_output s1 s2 s1_mod_eq s2_mod_eq (And.intro s1_init_step s1_star_s2_t)
+      match induct_star_res with
+      | ⟨t2, s3, P_true_tt2, s2_stars_s3_t2, no_inp_in_t2 ⟩ =>
+        exists t2
         constructor
-        . exact p1
-        . exists s3
-      . exact mainProof.right.right
+        . exact P_true_tt2
+        . constructor
+          . simp [behaviour]
+            have starComb := @star.trans_star _ _ (state_transition (NatModule.gcompf T f g)) s1 s2 s3 t t2 s1_star_s2_t s2_stars_s3_t2
+            exists s1
+            constructor
+            . exact s1_init_step
+            . exists s3
+          . exact no_inp_in_t2
